src/SepModels.v
@@ -1,0 +1,42 @@
+Require Import RelationClasses.
+Require Import SepTheory.
+Require Import Heaps.
+
+Set Implicit Arguments.
+Set Strict Implicit.
+
+Module Type SepModels (M : SeparationMemory) (ST : SepTheory).
+  Parameter aux : Type.
+
+  Parameter models : ST.hprop -> aux -> M.smem -> Prop.
+
+  Parameter models_pure : forall P a m,
+    models (ST.inj P) a m ->
+    P /\ models ST.emp a m.
+
+  Parameter models_star : forall P Q a m,
+    models (ST.star P Q) a m ->
+    exists m1 m2, M.split m m1 m2 /\
+        models P a m1 /\ models Q a m2.
+
+  Parameter models_ex : forall T (P : T -> ST.hprop) a m,
+    models (ST.ex P) a m ->
+    exists x : T, models (P x) a m.
+
+End SepModels.
+
+Module Type Foo (M : Memory) (SM : SeparationMemory with Module M := M).
+
+  Parameter models : SM.smem -> M.mem -> Prop.
+
+  Parameter memoryIn : M.mem -> SM.smem.
+
+  Parameter memoryIn_sound : forall m,
+    models (memoryIn m) m.
+
+  Parameter smem_get_sound : forall a v m sm,
+    models sm m ->
+    SM.smem_get a sm = Some v ->
+    M.mem_get m a = Some v.
+  
+  
